---
title: 'Mathematical Models of System<br />'
created: '2019-01-06T17:05:37.028Z'
author: 'Aditya Arora'
---
\newcommand{\N}{\mathbb{N}}
\newcommand{\Z}{\mathbb{Z}}
\newcommand{\C}{\mathbb{C}}
\newcommand{\R}{\mathbb{R}}
\newcommand{\iu}{{j\mkern1mu}}
\newcommand{\F}{\mathcal{F} }
\newcommand{\La}{\mathcal{L} }
\newcommand{\pd}{\partial }
\newcommand*{\ddo}[2]{\frac{d{#1}}{d{#2}}}
\newcommand*{\dt}[2]{\frac{d^2{#1}}{d{#2}^2}}
\newcommand*{\pdo}[2]{\frac{\pd{#1}}{\pd{#2}}}
\newcommand*{\pdt}[2]{\frac{\pd^2{#1}}{\pd{#2}^2}}
\newcommand*{\Co}[2]{\{#1\}\choose\{#2\}}
\newcommand*{\nbt}{\nabla^2}


for control design, we need a "good" (simple but accurate) mathematical model of how the plant responds to stimuli

## General comments on modelling
![dynamic system](../../attachments/dynamicsystem.png)

- a *model* is a set of equations that describe how a system transforms inputs into outputs
- no model is perfects (errors in measurement, approximations are made)
- models allow us to manipulate a system outside the constraints of physical reality
- in control: simple model for design, complex model for simulation

--- 
## Overview

1. Apply known laws to get a system of coupled differential equations
    - come from first principles eg: newton's, maxwell's, queuing theory, econometrics etc. and/or system identification (experiments, data fitting)
2. Linearize the model at an operating point to get a system of linear equations
    - simplify "linearize" model about an "operating point"
3. Take the Laplace transforms with zero initial conditions to get a system of linear algebraic equations
4. Isolate input and output to get a transfer function
    - express output $Y(s)$ in terms of the input $U(s)$
5. Experimentally determine parameter values for the transfer function (e.g. weight of your robot)

## Applying known laws to get equations
### e.g. Spring

![spring](../../attachments/spring.png)

$q(t) \in \mathbb{R}$ is the position of the mass $M$ at the time $t$, output

$M > 0$, mass in kg

$u$ - an externally applied force (input)

$\dot{q} := \frac{dq}{dt}, \quad \ddot{q} := \frac{d^2q}{dt^2}$

Assume that $q=0$ corresponds to the mass location at which the spring is neither stretched nor compressed - "unsprung".

Newton's 2nd law: $M\ddot{q} = \sum{ \text{forces acting on } M}$

Force due to spring: $F_K(q) = Kq(t)$, assumed to be linear, hooke's law

Force due to damper, possibly nonlinear: $C(\dot{q})$ where $C: \mathbb{R} \rightarrow \mathbb{R}$

Altogether, we get a second order nonlinear ODE:
$$M\ddot{q} = u(t) - Kq(t) - C(\dot{q})$$

Note: if the damper is linear ($C(\dot{q})=bq$), then the overall system is linear

### eg: 2 carts
![2 carts](../../attachments/2mass.png)

- a force $u$ is applied to $M_1$ and we want to control the position of $M_2$
- assume that when $q_1(t) = q_2(t)$, the spring is at rest

Applying Newton's second law on $M_1$ gives us two coupled second order linear ODEs: 
$$M_1\ddot{q_1} = u - Kq_1 + Kq_2 - b\dot{q}_1 + b\dot{q}_2$$
$$M_2\ddot{q_2} = Kq_1 - Kq_2 + b\dot{q}_1 - b\dot{q}_2$$

### e.g. Resistor

![resistor](../../attachments/resistor.png)
![V_r i graph](../../attachments/vr_i_graph.png)

$V_R(t) = h(i(t)), \quad h : \mathbb{R} \rightarrow \mathbb{R}$ is possibly nonlinear

$u(t)$: applied voltage; $y(t)$: voltage across capacitor

Apply Kirchoff's Voltage Law:
$$\begin{aligned}
-u(t) + V_R(t) + y(t) &= 0\\
\\
i(t) &= C\frac{dy}{dt} \quad \text{(capacitor equation)}\\
V_R &= h(i(t)) = h(C\dot(y))\\
\\
-u(t) + h(C\dot{y}) + y &= 0\\
\end{aligned}$$

Note: if the resister were linear ($h(i) = Ri$), the whole system would be linear (see 2.3.4 in notes)

> L02 Summary
> 
> - control design cycle (course roadmap)
> - Ch2 modelling
>   - examples - mech x2, elec x1
> 
> Expectation: model very simple, physical systems, see sec 2.3 of notes


## State-space models

a way to express mathematical models in standard form

### e.g. Cart
![carairresistance](../../attachments/carairresistance.png)

Newton's second law: $M\ddot{y} = u - D(\dot{y})$

We put this model into a standard form by defining two **state variables**:
$$x_1 := y \text{ (position)}, \quad x_2 := \dot{y} \text{ (velocity)}$$

Together, $x_1$ and $x_2$ make up the **state** of the system. We do some rewriting to have a systematic way to do linearization:

$$\begin{aligned}
\dot{x_1} &= x_2 & \text{(state equation)}\\
\dot{x_2} &= \frac{1}{M}u - \frac{1}{M}D(x_2) & \text{(state equation)}\\
y &= x_1 & \text{(output equation)}\\
\end{aligned}$$

Together, these equations make up the **state-space model.** These equations have the general form (also called the **Nonlinear state-space model**):

$$\dot{x} = f(x,u) \text{, } y = h(x(t))$$

In this example:

$$\begin{aligned}
x(t) &= \begin{bmatrix}
x_1(t) \\
x_2(t)\\
\end{bmatrix} \in \mathbb{R}^2\\
f(x,u) &= \begin{bmatrix}
x_2 \\
\frac{1}{M}u - \frac{1}{M}D(x_2)
\end{bmatrix}\\
\end{aligned}\\ h(x) = x_1$$

- the function $f: \mathbb{R}^2\times \mathbb{R} \rightarrow \R$ is linear if $D(x_2)$ is linear
-  $h: \mathbb{R}^2 \rightarrow \mathbb{R}$ is linear

In the special case where air resistance is a linear function of $x_2$ ($D(x_2)=d x_2$), then $f(x,u)$ becomes a linear function of $x$ and $u$:

$$f(x,u) = \begin{bmatrix}
0 & 1 \\
0 & \frac{-d}{M}
\end{bmatrix} \begin{bmatrix}
x_1 \\
x_2
\end{bmatrix} + \begin{bmatrix}
0 \\
\frac{1}{M}
\end{bmatrix} u
$$

Define $C = \begin{bmatrix}1 & 0\end{bmatrix}$. In the linear case, we get:
$$\begin{aligned}
\dot{x} &= Ax + Bu\\
y &= Cx\\
\end{aligned}$$

This is a linear, time-invariant (LTI) model.

**Expect at least one question like this on the midterm**

## Generalizing
Generalizing this example above, a large class of systems have models of the form:

$$\begin{aligned}
\dot{x} &= f(x, u), & f: \mathbb{R}^n \times \mathbb{R}^m \rightarrow \mathbb{R}^n\\
y &= h(x, u), & h: \mathbb{R}^n \times \mathbb{R}^m \rightarrow \mathbb{R}^p\\
\end{aligned}$$

- This model is nonlinear
- there are $m$ control inputs $u=(u_1, ..., u_m)$
- there are $p$ outputs $y=(y_1,...,y_p)$
- the state vector $x$ has dimensions $n$: $x=(x_1, ..., x_n)$

The LTI special case is:
$$\begin{aligned}
\dot{x} &= Ax + Bu, & A  \in \mathbb{R}^{n \times n}, B \in \mathbb{R}^{n \times m}\\
y &= Cx + Du, & C \in \mathbb{R}^{p \times n}, D \in \mathbb{R}^{p \times m}\\
\end{aligned}$$

### eg from previous example:

- n = 2
- m = 1 (one input-  applied force), 
- p = 1 (one output)

In this course, we look at single-input, single-output systems: $m=p=1$.

### e.g. more carts
![carts](../../attachments/carts.png)

$$\begin{aligned}
m&=2, & u &= (u_1, u_2)\\
p&=2, & y &= (y_1, y_2)\\
m&=4, & x &= (x_1, x_2, x_3, x_4) := (y_1, \dot{y_1}, y_2, \dot{y_2})\\
\end{aligned}$$

### e.g. drones
![drones](../../attachments/drones.png)
$$\begin{aligned}
m&= 4\\u &= (y_1, u_2, u_3, u_4)= (f_1, f_2, f_3, f_4)\\
p&=3\\
y&=(y_1, y_2, y_3)\\
n &= 12\\
x &\in \mathbb{R}^{12} = (\text{position}, \text{3 orientations - roll, pitch, and yaw}, \text{velocity}, \text{angular velocity})\\
\end{aligned}$$

### Determining state
**What is the state of a system?**

The state vector $x(t_0)$ encapsulates all of the system's evolution up to time $t_0$.

More formally: For any two times $t_0 \lt t$, knowing $x(t_0)$ and knowing $\{u(t) : t_0 \le t \le t_1\}$, we can compute $x(t_1)$ and hence $y(t_1)$.

> Faraz:System is causal

### e.g. cart with no forces
![cart-no-forces](../../attachments/cart-no-forces.png)

We know $M\ddot{y} = 0$ from Newton's laws.

If we try a 1-dimensional state, say $x := y$, then knowing $x(t_0)$ without knowing $\dot{y}$ is not enough information to find the position in the future, $x(t)$ for $t \gt t_0$. We have the same problem if we define $x = \dot{y}$.

Since the governing equation is second order, we need two initial conditions. So, $x=(y, \dot{y}) \in \mathbb{r}^2$ is a good choice.

In general, it is a good idea to use:

- position and velocity for a physical system
- Capacitor voltage and inductor current for a circuit

### e.g. 2.5.1: Pendulum

![pendulum](../../attachments/pendulum.png)

Model: $\ddot{\theta} = \frac{3}{Ml^2} u - 3\frac{g}{l} \sin(\theta)$

$$
\begin{aligned}
x &= \begin{bmatrix}
x_1 \\ x_2 
\end{bmatrix} := \begin{bmatrix}
\theta \\ \dot{\theta}
\end{bmatrix}\\
u &:= \tau \text{ (applied torque)}\\
y &:= \theta \text{ (position)}
\end{aligned}
$$

In state space form:
$$\begin{aligned}
x &= (\theta, \dot{\theta})\\
y &= \text{angular position} = \theta\\
\\
\dot{x}&=f(x,u) \quad & & \dot{x_1}=x_2\\
\dot{y}&=h(x,u) \quad & & \dot{x_2}=\frac{3}{Ml^2}u - 3\frac{s}{l} \sin(x_1)\\
& & & y = x_1
\end{aligned}$$

This is nonlinear due to the sine term, its state-space model *cannot* be written in the form as above

### e.g. 2.4.5 Circuit
![circuit](../../attachments/circuit.png)

$$
\begin{aligned}
x &= \begin{bmatrix}
x_1 \\ x_2 
\end{bmatrix} := \begin{bmatrix}
\text{voltage across cap} \\ \text{current through inductor}
\end{bmatrix}\\
u &:= \text{ (applied voltage)}\\
y &:= \text{current through inductor}
\end{aligned}
$$

$$\begin{aligned}
x_1 &:= \text{voltage across capacitor} = \frac{1}{C} \int{y(\tau)d\tau}\\
x_2 &:= \text{current through inductor} = y\\
\\
-u + V_R + V_C + V_L &= 0\\
\Rightarrow -u + Rx_2  + x_1 + L\dot{x_2} &= 0, \quad \text{from capacitor equation: } \dot{x_1}=\frac{1}{C} x_2\\
\\
\dot{x} &= \begin{bmatrix}
0 & \frac{1}{C}\\
\frac{-1}{2} & \frac{-R}{L}\end{bmatrix} \begin{bmatrix}x_1\\
x_2\end{bmatrix} + \begin{bmatrix}0 \\ \frac{1}{L}\end{bmatrix} u\\
y &= \begin{bmatrix}0 & 1\end{bmatrix}\\
\end{aligned}$$

The above is a linear system, and right above this is the state space model

> L03 summary 
> 
> ![](../../attachments/L03_summary.png)
> 
> Non-linear time-invariant causal state-space model
> $$ \begin{aligned}
f&: \R^n \times \R^m \to \R^n\\
h&: \R^n \times \R^m \to \R^p
\end{aligned}
$$
> Single-input single output: m = p = 1
> 
> State vector: $z(t)$, given $x(t_0)$ and $u(t), t_0 \leq t \leq t_1$, we can compute $y(t_1)$
> 
> Rule of thumb: 
> 1. mechanical - posn and velocity
> 2. electrical: Inductor currents and capacitor voltages
> 
> **LTI SPECIAL CASE**
> 
> ![](../../attachments/L03_summary.png)
> 
> $A \epsilon \R^{n\times n};B \epsilon \R^{n\times m};C \epsilon \R^{p\times n};D \epsilon \R^{p\times n};$

## Linearization
In this course we always linearize, non-linear system

This refers to the process of approximating a nonlinear state-space model with a linear model

Linearization allows us to use simpler, systematic analysis and design tools

### e.g. 2.5.2
Linearize $y=x^3$ at the point $\bar{x}=1$.

![linearize](../../attachments/linearize.png)

Let $\bar{y} := f(\bar{x}) = 1^3 = 1$

Taylor series at $x=\bar{x}$ is:
$$y=\sum_{n=0}^\infty c_n (x-\bar{x})^n, \quad c_n = \frac{1}{n!} \frac{d^n f(x)}{dx^n} \biggr|_{x=\bar{x}}$$

Keep only the terms $n=0$ and $n=1$:
$$\begin{aligned}
f(x) &\approx f(\bar{x}) + \frac{df(x)}{dx}\biggr|_{x-\bar{x}} (x-\bar{x})\\
y - \bar{y} &\approx + \frac{df(x)}{dx}\biggr|_{x-\bar{x}} (x-\bar{x})\\
\end{aligned}$$

If we define the derivations $\partial y := y - \bar{y}, \partial x := x - \bar{x}$, then $\partial y = \frac{df}{dx} \bigg|_{x=\bar{x}} \partial x$, i.e. $\partial y = 3 \partial x$

### e.g. 2.5.3
$$y = \begin{bmatrix}y_1 \\ y_2\end{bmatrix} = f(x) = \begin{bmatrix}x_1 x_2 - 1 \\ x_3^2 - 2x_1 x_3\end{bmatrix} =: \begin{bmatrix}f_1(x) \\ f_2(x)\end{bmatrix}$$

Linearize at $\bar{x}=(1, -1, 2)$.

$\bar{y}=f(\bar{x})=\begin{bmatrix}-2\\0\end{bmatrix}$

### Multivariable Taylor series
$$d(x)=f(\bar{x})+\frac{\partial f}{\partial x} \biggr|_{x=\bar{x}} (x-\bar{x}) \text{ + higher order terms}$$

The Jacobian of $f$ at $\bar{x}$ is:
$$\begin{aligned}
\frac{\partial f}{\partial x} \biggr|_{x = \bar{x}}
&= \begin{bmatrix}
  \frac{\partial f_1}{\partial x_1} & \frac{\partial f_1}{\partial x_2} & \frac{\partial f_1}{\partial x_3} \\
  \frac{\partial f_2}{\partial x_1} & \frac{\partial f_2}{\partial x_2} & \frac{\partial f_2}{\partial x_3} \\
  \frac{\partial f_3}{\partial x_1} & \frac{\partial f_3}{\partial x_2} & \frac{\partial f_3}{\partial x_3} \\
\end{bmatrix}\\
&= \begin{bmatrix}
  x_2 & x_1 & 0 \\
  -2x_3 & 0 & 2x_3-2x_1 \\
\end{bmatrix}_{x=(1, -1, 2)}\\
&= \begin{bmatrix}
  -1 & 1 & 0\\
  -4 & 0 & 2
\end{bmatrix}\\
&= A
\end{aligned}$$

i.e. $y-\bar{y} \approx A(x-\bar{x})$

You can now think of this as tangent planes to surfaces

By direect extension, at $(x,u)=(\bar{x}, \bar{u})$:
$$f(x, u) \approx f(\bar{x}, \bar{u})+ \frac{\partial f}{\partial x} \biggr|_{(x,u)=(\bar{x}, \bar{u})} (x-\bar{x}) + \frac{\partial f}{\partial u} \biggr|_{(x,u)=(\bar{x}, \bar{u})} (u-\bar{u})$$



Let's apply linearization to $\dot{x}=f(x,u), y=h(x,u)$.

**Definition (2.5.1):** A constant pair $(\bar{x}, \bar{u}) \in \mathbb{R}^n \times \mathbb{R}^m$ is an **equilibrium configuration** of the system $\dot{x}=f(x,u), y=h(x,u)$ if $f(\bar{x}, \bar{u})=(0,...,0)$. The constant $\bar{x}$ is the **equilibrium point.**

### e.g. Find all the equilibria at which the pendulum is upright

$$\begin{aligned}
\dot{x} &= f(x,u)\\
y &= h(x,u)\\
x_1 &= \theta\\
x_2 &= \dot{\theta}\\
f(x,u) &= \begin{bmatrix}x_2\\ \frac{3}{Ml}u-\frac{3g}{l}\sin(x_1)\end{bmatrix}\\
h(x) &= x_1
\end{aligned}$$

If $y=\pi$ (upright), then $\bar{x_1}=\pi$. So we have to solve:
$$
\begin{bmatrix}0\\0\end{bmatrix} = \begin{bmatrix}
  \bar{x_2}\\
  \frac{3\bar{u}}{Ml} - \frac{3g}{l}\sin(\bar{x_1})
\end{bmatrix} \Rightarrow \bar{x_2}=0, \quad \bar{u}=0
$$

Therefore the equilibria are:
$$
\begin{bmatrix}\bar{x_1}\\\bar{x_2}\end{bmatrix} = \begin{bmatrix}\pi + 2\pi k \\ 0\end{bmatrix}, \quad \bar{u}=0
$$

Assume that $\dot{x}=f(x,u)$ has an equilibrium configuration at $(x,u)=(\bar{x}, \bar{u})$.

$$
f(x,u) \approx \underbrace{f(\bar{x}, \bar{u})}_{=0} + \underbrace{\frac{\partial f}{\partial x} \biggr|_{(x,u)=(\bar{x}, \bar{u})} (x - \bar{x})}_{=: A} + \underbrace{\frac{\partial f}{\partial u} \biggr|_{(x,u)=(\bar{x}, \bar{u})} (u - \bar{u})}_{=:B}$$

Consider deviations from $(\bar{x}, \bar{u})$, where $||\partial x||, ||\partial u||$ are assumed to be small:
$$\begin{aligned}
\partial x(t) &:= x(t) - \bar{x}\\
\partial u(t) &:= u(t) - \bar{u}\\
\end{aligned}$$

Then we get linearized state equations:
$$\dot{\partial x} = \dot{x} - 0 = f(x,u) \approx A\partial x + B \partial u\\
\dot{\partial x} = A\partial x + B\partial u$$

Linearized output equation:

$$\partial y = \underbrace{\frac{\partial h}{\partial x} \biggr|_{(x,u)=(\bar{x},\bar{u})} \partial x}_{=:C} + \underbrace{\frac{\partial h}{\partial u} \biggr|_{(x,u)=(\bar{x},\bar{u})} \partial u}_{=:D}\\
\partial y := y-\bar{y}=y-h(\bar{x},\bar{u})$$

### Obtaining a Transfer function from a state-space model

- start w/ an LTI state-space model
$$
\dot{\partial x(t)} = A\partial x + B\partial y\\
y(t) = Cx(t) + Dy(t)
$$
- take LTs w/ zero initial conditions 
$$
sX(s) = AX(s) + BU(s)\\
Y(s) = CX(s) + DU(s)
$$
$$X(s) = \begin{bmatrix}
X_1(s)\\
\vdots\\
X_n(s)
\end{bmatrix}
$$
$$U(s) = \begin{bmatrix}
U_1(s)\\
\vdots\\
U_m(s)
\end{bmatrix}
$$
$$Y(s) = \begin{bmatrix}
Y_1(s)\\
\vdots\\
Y_p(s)
\end{bmatrix}
$$
- eliminate $X(S)$
$$
\begin{aligned}
(sI - A)X(s) &= BU(s) \\
X(s) &= (sI - A)^{-1}BU(s)\\
Y(s) &= \underbrace{(C(sI - A)^{-1}B + D)}_{G(s)}U(s)
\end{aligned}
$$
$G(s)$ is the transfer function

#### Summary: Getting a transfer function

1. Use first principles to obtain the ODEs that govern the system's behaviour. Put into state-space form
2. Pick an equilibrium configuration $(\bar{x}, \bar{u})$ typically depends on a desired output $\bar{y}$ around which we wish to control the plant
3. Linearize $(\bar{x}, \bar{u})$ to get $A, B, C, D$
4. Transfer Function: $G(s) = (sI - A)^{-1}B$ MATLAB: `ss|tf`

##### Ex: 2.8.6 Recall the linearized model of the pendulum in the upright position

$$\begin{aligned}
\partial \dot{x} &= \begin{bmatrix} 0 & 1 \\ \frac{3g}{2l} & 0 \end{bmatrix} \partial x + \begin{bmatrix}0 \\ \frac{3}{Ml^2}\end{bmatrix} \partial u\\
\partial y &= \begin{bmatrix}1 & 0\end{bmatrix} \partial x\\
\\
G(s) &= C(sI-A)^{-1}B + D, \quad (sI-A)^{-1} = \frac{\text{adj}(sI-A)}{\det(sI-A)}\\
&= \begin{bmatrix}1 & 0\end{bmatrix}\begin{bmatrix}s & -1 \\ \frac{-3g}{2l} & s\end{bmatrix}^{-1}\begin{bmatrix}0 \\ \frac{3}{Ml^2}\end{bmatrix}\\
&= \frac{\begin{bmatrix}1 & 0\end{bmatrix}\begin{bmatrix}s & \frac{3g}{2l} \\ 1 & s\end{bmatrix}^T\begin{bmatrix}0 \\ \frac{3}{Ml^2}\end{bmatrix}}{s^2 - 1.5\frac{g}{l}}\\
&= \frac{3}{(Ml^2)(s^2 - \frac{1.5g}{l})}\\
\end{aligned}$$

#### Summary 

1. Select an equilibrium configuration $(\bar{x}, \bar{u}) \in \mathbb{R}^n \times \mathbb{R}^m$: $\bar{y}=h(\bar{x},\bar{u}), f(\bar{x},\bar{u})=0$
2. Compute Jacobians of $f,h$ to get $A,B,C,D$
3. Linearization: $\dot{\partial x} = A \partial + B \partial u, \partial y = C \partial x + D \partial u$

## Block diagram manipulations
```
          +------+
  U(s) -->| G(s) |--> Y(s)      Y(s) = G(s)U(s)
          +------+

           +------+
        +->| G(s) |--+
        |  +------+  |
  U(s) -+            +--> Y(s)   Y(s) = (G(s) + H(s))U(s)
        |  +------+  |
        +->| H(s) |--+
           +------+

                                        D(s) 
                                         |
                                         v
                                      +-----+
                  D(s)                | 1/G |
                    |                 +-----+   
          +------+  v                     |   +------+
  U(s) -->| G(s) |--o--> Y(s)   =  U(s) --o-->| G(s) |   Y(s) = D(s) + G(s)U(s)
          +------+                            +------+


             +------+
  U(s) --o-->| G(s) |--+--> Y(s)      Y(s) = G(s)U(s)/(1 + G(s)H(s))
         ^-  +------+  |
         |             |
         |   +------+  |
         +---| H(s) |--+
             +------+ 

```

### e.g. Linearized pendulum
Find the transfer function from $U$ to $Y$

![model](../../attachments/model.jpg)

#### Strategy 1: Express Y directly in terms of U and simplify
$$\begin{aligned}
Y(s) &= G_2(s) (G_{ff}(s) U(s) + G_1(s) (U(s) - Y(s)))\\
\frac{Y(s)}{U(s)} = \frac{G_2G_{ff} + G_2G_1}{1 + G_2G_1}
\end{aligned}
$$

#### Strategy 2: Re-arrange block to reveal common configurations

- move $G_1$ to the left of negative feedback junction and swap locations of the negative feedback junction, and the positive feed forward junction\
![model_rearranged](../../attachments/model_rearranged.jpg)
- Now we have a parallel connection in series with a negative feedback connection

$$
Y(s) = (G_{ff} + G_1)(\frac{G_2}{1 + GG_2})
$$


## Systematic method of finding transfer functions
1. Introduce new signals $\{v_1, v_2, ... \}$ at the output of every summing junction
2. Write expressions for inputs of summers in terms of $\{u, y, v_1, v_2, \dots\}$
3. Write equations for each summer and $y$
4. Eliminate $\{v_1, v_2, ...\}$ from equations

e.g.
![blockdiagramtf](../../attachments/blockdiagramtf.png)

$$\begin{aligned}
y&=G_3G_2v_2\\
v_2 &= H_2y+G_1v_1-H_2G_2v_1\\
v_1&=u-H_1G_2v_2\\
\\
\begin{bmatrix}1 & H_1 G_2 & 0 \\ -G_1 & 1+H_2G_2 & -H_3 \\ 0 & -G_3G_2 & 1\end{bmatrix}
  \begin{bmatrix}v_1 \\ v_2 \\ y\end{bmatrix} &= \begin{bmatrix}u \\ 0 \\ 0\end{bmatrix}\\
\\
\text{By cramer's rule:}\\
Y(s) &- \frac{
\det\begin{bmatrix}1 & H_1G_2 & u \\ -G_1 & 1+H_2G_2 & 0 \\ 0 & -G_2G_3 & 0\end{bmatrix}
}{
\det\begin{bmatrix}1 & H_1G_2 & 0 \\ -G_1 & 1+H_2G_2 & -H_3 \\ 0 & -G_3G_2 & 1\end{bmatrix}
}\\
&= \frac{G_1 G_2 G_3}{1 + H_1 H_2 G_2 - H_3 G_3 G_2 + G_1 H_1 G_2} U(s)\\
\end{aligned}$$


